refactor definitions and add fairness

epfd/Epfd/Basic.lean
@@ -12,14 +12,21 @@ import Mathlib.Data.Finset.Basic
 -- The abstract type of processes
 variable (Proc : Type) [DecidableEq Proc] [Hashable Proc] [Repr Proc]
 
--- The global stabilization time GST, unknown to the processes
+inductive MsgTag where
+  | HeartbeatRequest
+  | HeartbeatReply
+  deriving DecidableEq, Repr
+
 /-- A message that is sent by one process (src) to another process (dst).
     Every message is equipped with a timestamp, which is equal to the
     clock value at the time of sending the message.
  -/
-inductive Message where
-  | HeartbeatRequest (src: Proc) (dst: Proc) (timestamp: Nat)
-  | HeartbeatReply (src: Proc) (dst: Proc) (timestamp: Nat)
+@[ext]
+structure Msg where
+  kind: MsgTag
+  src: Proc
+  dst: Proc
+  timestamp: ℕ
   deriving DecidableEq, Repr
 
 /-- A global state of the eventually perfect failure detector:
@@ -29,7 +36,7 @@ inductive Message where
   - `suspected` is a map from each process to the set of processes that it
     considers suspected.
   - `delay` is a map from each process to its delay (in clock units).
-  - `msgs` is the set of messages that have been sent by the processes.
+  - `sent` is the set of messages that have been sent by the processes.
   - `rcvd` is the set of messages that have been received by the processes.
   - `clock` is a global clock value.
   - `crashed` is the set of processes that have actually crashed.
@@ -41,8 +48,8 @@ structure ProtocolState where
   -- It may differ from run to run, but remains constant during a run.
   all: Finset Proc
   crashed: Finset Proc
-  msgs: Finset (@Message Proc)
-  rcvd: Finset (@Message Proc)
+  sent: Finset (Msg Proc)
+  rcvd: Finset (Msg Proc)
   clock: Nat
   alive: Std.HashMap Proc (Finset Proc)
   suspected: Std.HashMap Proc (Finset Proc)
@@ -52,30 +59,29 @@ structure ProtocolState where
 /--
   Given a message that was sent at `timestamp`, can a process receive it at time `clock`.
   -/
-def isMessageTimely (GST: Nat) (MsgDelay: Nat) (timestamp: Nat) (clock: Nat): Bool :=
-    timestamp ≥ GST && clock ≥ timestamp && clock ≤ timestamp + MsgDelay
-  || timestamp < GST && clock ≥ timestamp
+def isMsgTimely (GST: Nat) (MsgDelay: Nat) (timestamp: Nat) (clock: Nat): Bool :=
+  clock ≥ timestamp && clock ≤ (max GST timestamp) + MsgDelay
 
 example:
   -- After GST, clock must be within [timestamp, timestamp + MsgDelay]
   -- GST = 100, MsgDelay = 5, timestamp = 120, clock = 121
-  @isMessageTimely 100 5 120 121 == true := rfl
+  @isMsgTimely 100 5 120 121 == true := rfl
 
 example:
   -- After GST, clock must be within [timestamp, timestamp + MsgDelay]
   -- GST = 100, MsgDelay = 5, timestamp = 120, clock = 127
-  @isMessageTimely 100 5 120 127 == false := rfl
+  @isMsgTimely 100 5 120 127 == false := rfl
 
 example:
   -- Before GST, we can receive a message much later
   -- GST = 100, MsgDelay = 5, timestamp = 21, clock = 50
-  @isMessageTimely 100 5 21 50 == true := rfl
+  @isMsgTimely 100 5 21 50 == true := rfl
 
 example:
   -- We cannot receive a message earlier than it was sent,
   -- either before or after GST.
   -- GST = 100, MsgDelay = 5, timestamp = 21, clock = 20
-    @isMessageTimely 100 5 21 20 == false
+    @isMsgTimely 100 5 21 20 == false
   -- GST = 100, MsgDelay = 5, timestamp = 121, clock = 120
-  ∧ @isMessageTimely 100 5 121 120 == false
+  ∧ @isMsgTimely 100 5 121 120 == false
     := by apply And.intro; rfl; rfl
